iris/WpAuipc.v
@@ -1,0 +1,253 @@
+(* WpAuipc.v -- the AUIPC opcode: execute reduction, forward_exec_auipc, wp_step_auipc. *)
+From Stdlib Require Import Eqdep_dec ZArith Lia.
+From stdpp Require Import gmap list list_monad bitvector.definitions bitvector.tactics.
+From iris.proofmode Require Import proofmode.
+From iris.base_logic.lib Require Import gen_heap.
+From iris.program_logic Require Import language weakestpre lifting.
+Require Import SailStdpp.ConcurrencyInterface SailStdpp.ConcurrencyInterfaceBuiltins SailStdpp.ConcurrencyInterfaceTypes SailStdpp.Operators_mwords.
+Require Import Riscv.rv64d_types Riscv.rv64d.
+Require Import RiscvModelBytes.
+Require Import SailStdpp.Base SailStdpp.TypeCasts.
+Require Import Riscv.rv64d_types Riscv.rv64d.
+Require Import RiscvLang RiscvPtsto RiscvExec RiscvTryStep RiscvFetchExec RiscvExtras WpAdd.
+Local Open Scope Z_scope.
+Import Defs.
+
+(* --- get_arch_pc reads PC (state-pure). --- *)
+Lemma run_get_arch_pc s :
+  run (get_arch_pc tt) s (register_lookup PC s.(sregs)) s.
+Proof. unfold get_arch_pc. exact (run_read_reg_fwd PC s). Qed.
+
+Lemma exec_get_arch_pc s :
+  exec (get_arch_pc tt) s = Some (register_lookup PC s.(sregs), s).
+Proof. unfold get_arch_pc. exact (exec_read_reg PC s). Qed.
+
+(* --- execute (UTYPE imm rd AUIPC): read PC, add imm<<12, write rd, retire. --- *)
+Definition auipc_off (imm : mword 20) : mword 64 :=
+  sign_extend' 64 (concat_vec imm (Ox"000")).
+
+Lemma exec_execute_UTYPE_AUIPC (i : mword 5) (imm : mword 20) s :
+  uint i = 2 ->
+  exec (execute_UTYPE imm (Regidx i) AUIPC) s
+  = Some (RETIRE_SUCCESS,
+          set_reg s (R_bitvector_64 x2)
+            (regval_into_reg
+               (add_vec (register_lookup PC s.(sregs)) (auipc_off imm)))).
+Proof.
+  intro Hi.
+  unfold execute_UTYPE, auipc_off. cbn match.
+  rewrite (exec_bind_Some _ _ _
+             (add_vec (register_lookup PC s.(sregs))
+                      (sign_extend' 64 (concat_vec imm (Ox"000")))) s).
+  2:{ rewrite (exec_bind_Some _ _ _ _ _ (exec_get_arch_pc s)). apply exec_returnm. }
+  rewrite (exec_bind0_Some _ _ _ _ _ (exec_wX_bits_x2 i s _ Hi)). apply exec_returnm.
+Qed.
+
+(* ---------------------------------------------------------------------- *)
+(* forward_exec_auipc: thread the generic try_step wrapper + the generic    *)
+(* run_hart_active progress engine around the AUIPC execute leaf.           *)
+(* Hypotheses mirror forward_exec_final's: universally-quantified fetch /    *)
+(* decode / should_inc facts + booting-Machine register conditions.         *)
+(* ---------------------------------------------------------------------- *)
+
+Section ForwardAUIPC.
+  Context (s : mstate) (w : mword 32) (pc : mword 64) (imm : mword 20)
+          (i : mword 5) (b : bool).
+
+  Hypothesis Hi : uint i = 2.
+  Hypothesis Hfetch_gen : forall s0 : mstate,
+    register_lookup PC s0.(sregs) = pc ->
+    register_lookup cur_privilege s0.(sregs) = Machine ->
+    exec (fetch tt) s0 = Some (F_Base w, s0).
+  Hypothesis Hdec_gen : forall s0 : mstate,
+    exec (ext_decode w) s0 = Some (UTYPE (imm, Regidx i, AUIPC), s0).
+  Hypothesis Hsi_s : exec (should_inc_minstret Machine) s = Some (b, s).
+
+  Definition sAa : mstate := set_reg s (R_bool minstret_increment) b.
+  Definition sXa : mstate :=
+    let s1 := set_reg sAa nextPC (add_vec_int pc 4) in
+    set_reg s1 (R_bitvector_64 x2)
+      (regval_into_reg (add_vec (register_lookup PC s1.(sregs)) (auipc_off imm))).
+  Definition sTa : mstate := set_reg sXa PC (register_lookup nextPC sXa.(sregs)).
+  Definition sFa : mstate :=
+    if b then set_reg sTa minstret
+                  (add_vec_int (register_lookup minstret sTa.(sregs)) 1)
+         else sTa.
+
+  Lemma forward_exec_auipc :
+    register_lookup PC s.(sregs) = pc ->
+    register_lookup cur_privilege s.(sregs) = Machine ->
+    register_lookup hart_state s.(sregs) = HART_ACTIVE tt ->
+    register_lookup (R_bitvector_64 mideleg) s.(sregs) = zeros' 64 ->
+    eq_vec (_get_Mstatus_MIE (register_lookup (R_bitvector_64 mstatus) s.(sregs)))
+           ('b"1") = false ->
+    eq_vec (register_lookup elp s.(sregs)) (landing_pad_bits_backwards LP_EXPECTED) = false ->
+    exec riscv_step s = Some (tt, sFa).
+  Proof using All.
+    intros Lpc Lpriv Lhs Lmideleg LmIE Lelp.
+    (* booting-config reads transfer through the minstret_increment write. *)
+    assert (LpcA  : register_lookup PC sAa.(sregs) = pc).
+    { unfold sAa, set_reg; cbn [sregs]. rewrite irrelevant_register_set;
+        [ exact Lpc | vm_compute; reflexivity ]. }
+    assert (LprivA: register_lookup cur_privilege sAa.(sregs) = Machine).
+    { unfold sAa, set_reg; cbn [sregs]. rewrite irrelevant_register_set;
+        [ exact Lpriv | vm_compute; reflexivity ]. }
+    assert (LhsA  : register_lookup hart_state sAa.(sregs) = HART_ACTIVE tt).
+    { unfold sAa, set_reg; cbn [sregs]. rewrite irrelevant_register_set;
+        [ exact Lhs | vm_compute; reflexivity ]. }
+    assert (LmidA : register_lookup (R_bitvector_64 mideleg) sAa.(sregs) = zeros' 64).
+    { unfold sAa, set_reg; cbn [sregs]. rewrite irrelevant_register_set;
+        [ exact Lmideleg | vm_compute; reflexivity ]. }
+    assert (LmIEA : eq_vec (_get_Mstatus_MIE
+              (register_lookup (R_bitvector_64 mstatus) sAa.(sregs))) ('b"1") = false).
+    { unfold sAa, set_reg; cbn [sregs]. rewrite irrelevant_register_set;
+        [ exact LmIE | vm_compute; reflexivity ]. }
+    assert (LelpA : eq_vec (register_lookup elp sAa.(sregs))
+              (landing_pad_bits_backwards LP_EXPECTED) = false).
+    { unfold sAa, set_reg; cbn [sregs]. rewrite irrelevant_register_set;
+        [ exact Lelp | vm_compute; reflexivity ]. }
+    (* dispatchInterrupt = None at sAa via the getPendingSet keystone;
+       currentlyEnabled Ext_S reduces for any state (exec_currentlyEnabled_S). *)
+    assert (HdispA : exec (dispatchInterrupt Machine) sAa = Some (None, sAa)).
+    { apply exec_dispatchInterrupt_none.
+      apply (exec_getPendingSet_machine_none sAa _ (exec_currentlyEnabled_S sAa) LmidA LmIEA). }
+    (* fetch / decode at sAa (state-preserving). *)
+    assert (HfetchA : exec (fetch tt) sAa = Some (F_Base w, sAa))
+      by (apply Hfetch_gen; assumption).
+    assert (HdecA : exec (ext_decode w) sAa = Some (UTYPE (imm, Regidx i, AUIPC), sAa))
+      by apply Hdec_gen.
+    (* execute leaf at s_pc = set_reg sAa nextPC (pc+4). *)
+    pose (s_pc := set_reg sAa nextPC (add_vec_int pc 4)).
+    assert (HpcPCpc : register_lookup PC s_pc.(sregs) = pc).
+    { unfold s_pc, set_reg; cbn [sregs]. rewrite irrelevant_register_set;
+        [ exact LpcA | vm_compute; reflexivity ]. }
+    assert (HexecA : exec (execute (UTYPE (imm, Regidx i, AUIPC))) s_pc
+              = Some (RETIRE_SUCCESS, sXa)).
+    { change (execute (UTYPE (imm, Regidx i, AUIPC)))
+        with (execute_UTYPE imm (Regidx i) AUIPC).
+      unfold sXa. fold s_pc.
+      exact (exec_execute_UTYPE_AUIPC i imm s_pc Hi). }
+    (* the run_hart_active reduction (exact value) via the generic engine. *)
+    assert (Hha : exec (run_hart_active 0) sAa
+              = Some (Step_Execute (RETIRE_SUCCESS, zero_extend' 32 w), sXa)).
+    { exact (exec_hart_active_progress sAa sAa sXa sAa w
+               (UTYPE (imm, Regidx i, AUIPC)) pc RETIRE_SUCCESS
+               LprivA HdispA HfetchA HdecA LelpA ltac:(reflexivity) LpcA HexecA I). }
+    (* the generic try_step wrapper. *)
+    apply (exec_riscv_step_ADD s sXa w b pc).
+    - exact Lpriv.
+    - exact Hsi_s.
+    - exact LhsA.
+    - exact Hha.
+    - (* hart_state at sXa = HART_ACTIVE tt *)
+      unfold sXa, sAa; cbn zeta. trans_mi. trans_mi. trans_mi. exact Lhs.
+    - (* minstret_increment at sXa = b *)
+      unfold sXa, sAa; cbn zeta. trans_mi. trans_mi.
+      rewrite register_lookup_set. reflexivity.
+    - reflexivity. (* Hrvfi : get_config_rvfi tt = false -- definitional *)
+  Qed.
+
+  (* clean-form post-state (concrete values), mirror of base_upd/sFc/sF_eq. *)
+  Variable mst0 : mword 64.
+  Hypothesis Lmst_a : register_lookup minstret s.(sregs) = mst0.
+
+  Definition base_upd_a : mstate :=
+    set_reg (set_reg (set_reg (set_reg s (R_bool minstret_increment) b)
+                              nextPC (add_vec_int pc 4))
+                     (R_bitvector_64 x2) (regval_into_reg (add_vec pc (auipc_off imm))))
+            PC (add_vec_int pc 4).
+  Definition sFca : mstate :=
+    if b then set_reg base_upd_a minstret (add_vec_int mst0 1)
+         else base_upd_a.
+
+  Ltac tmiss := rewrite irrelevant_register_set; [ | vm_compute; reflexivity ].
+
+  Lemma sFa_eq : register_lookup PC s.(sregs) = pc -> sFa = sFca.
+  Proof.
+    intro LpcS.
+    assert (Enpc : register_lookup nextPC sXa.(sregs) = add_vec_int pc 4).
+    { unfold sXa; cbv zeta. unfold set_reg; cbn [sregs]. tmiss.
+      rewrite register_lookup_set. reflexivity. }
+    assert (Epc1 : register_lookup PC (set_reg sAa nextPC (add_vec_int pc 4)).(sregs) = pc).
+    { unfold sAa, set_reg; cbn [sregs]. tmiss. tmiss. exact LpcS. }
+    assert (HsT : sTa = base_upd_a).
+    { unfold sTa. rewrite Enpc. unfold sXa; cbv zeta. rewrite Epc1.
+      unfold regval_into_reg, base_upd_a, sAa. reflexivity. }
+    unfold sFa, sFca. rewrite HsT. destruct b; [|reflexivity].
+    assert (Emst : register_lookup minstret base_upd_a.(sregs) = register_lookup minstret s.(sregs)).
+    { unfold base_upd_a, set_reg; cbn [sregs]. tmiss. tmiss. tmiss. tmiss. reflexivity. }
+    rewrite Emst Lmst_a. reflexivity.
+  Qed.
+
+End ForwardAUIPC.
+
+Section StepAUIPC.
+  Context `{!riscvGS Σ}.
+  Lemma wp_step_auipc (pc : mword 64) (w_a : mword 32) (imm_a : mword 20)
+      (i_a : mword 5) (b1 : bool) (sp0a npc0a mst0a mstatus0a : mword 64)
+      (mc : mword 32) (mcfg : mword 64)
+      (mi0a : bool) (elp0a : mword 1) E (Φ : mval -> iProp Σ) :
+    uint i_a = 2 ->
+    (forall s0, register_lookup PC s0.(sregs) = pc ->
+       register_lookup cur_privilege s0.(sregs) = Machine ->
+       exec (fetch tt) s0 = Some (F_Base w_a, s0)) ->
+    (forall s0, exec (ext_decode w_a) s0 = Some (UTYPE (imm_a, Regidx i_a, AUIPC), s0)) ->
+    (* should_inc is now DETERMINED by the mcountinhibit/minstretcfg cells: *)
+    b1 = andb (eq_vec (_get_Counterin_IR mc) ('b"0"))
+              (eq_vec (counter_priv_filter_bit mcfg Machine) ('b"0")) ->
+    eq_vec (_get_Mstatus_MIE mstatus0a) ('b"1") = false ->
+    eq_vec elp0a (landing_pad_bits_backwards LP_EXPECTED) = false ->
+    PC ↦ᵣ pc -∗ (R_bitvector_64 x2) ↦ᵣ sp0a -∗ nextPC ↦ᵣ npc0a -∗
+    (R_bool minstret_increment) ↦ᵣ mi0a -∗ minstret ↦ᵣ mst0a -∗
+    cur_privilege ↦ᵣ Machine -∗ hart_state ↦ᵣ HART_ACTIVE tt -∗
+    (R_bitvector_64 mideleg) ↦ᵣ zeros' 64 -∗ (R_bitvector_64 mstatus) ↦ᵣ mstatus0a -∗
+    elp ↦ᵣ elp0a -∗ mcountinhibit ↦ᵣ mc -∗ minstretcfg ↦ᵣ mcfg -∗
+    ▷ ( PC ↦ᵣ add_vec_int pc 4 -∗
+        (R_bitvector_64 x2) ↦ᵣ regval_into_reg (add_vec pc (auipc_off imm_a)) -∗
+        nextPC ↦ᵣ add_vec_int pc 4 -∗ (R_bool minstret_increment) ↦ᵣ b1 -∗
+        minstret ↦ᵣ (if b1 then add_vec_int mst0a 1 else mst0a) -∗
+        cur_privilege ↦ᵣ Machine -∗ hart_state ↦ᵣ HART_ACTIVE tt -∗
+        (R_bitvector_64 mideleg) ↦ᵣ zeros' 64 -∗ (R_bitvector_64 mstatus) ↦ᵣ mstatus0a -∗
+        elp ↦ᵣ elp0a -∗ mcountinhibit ↦ᵣ mc -∗ minstretcfg ↦ᵣ mcfg -∗
+        WP (Loop : expr riscv_lang) @ E {{ Φ }}) -∗
+    WP (Loop : expr riscv_lang) @ E {{ Φ }}.
+  Proof.
+    iIntros (Hia Hfa Hda Hb1 HmIE Help) "Hpc Hx2 Hnpc Hmi Hmst Hpriv Hhs Hmdl Hms Help Hmcinh Hmcfg Hcont".
+    iApply wp_exec_step. iIntros (s ns κs nt) "[Hreg Hmem]".
+    iDestruct (reg_valid with "Hreg Hpc")    as %Lpc.
+    iDestruct (reg_valid with "Hreg Hpriv")  as %Lpriv.
+    iDestruct (reg_valid with "Hreg Hhs")    as %Lhs.
+    iDestruct (reg_valid with "Hreg Hmdl")   as %Lmdl.
+    iDestruct (reg_valid with "Hreg Hms")    as %Lms.
+    iDestruct (reg_valid with "Hreg Hmst")   as %Lmst.
+    iDestruct (reg_valid with "Hreg Help")   as %Lelp.
+    iDestruct (reg_valid with "Hreg Hmcinh") as %Lmc.
+    iDestruct (reg_valid with "Hreg Hmcfg")  as %Lmcfg.
+    assert (Hsi_s : exec (should_inc_minstret Machine) s = Some (b1, s)).
+    { rewrite Hb1. apply (exec_should_inc_M mc mcfg s Lmc Lmcfg). }
+    iApply fupd_mask_intro; [set_solver|]. iIntros "Hclose".
+    iExists (sFca s pc imm_a b1 mst0a). iSplitR.
+    { iPureIntro.
+      rewrite <- (sFa_eq s pc imm_a b1 Hsi_s mst0a Lmst Lpc).
+      apply (forward_exec_auipc s w_a pc imm_a i_a b1 Hia Hfa Hda Hsi_s Lpc Lpriv Lhs Lmdl).
+      - rewrite Lms. exact HmIE.
+      - rewrite Lelp. exact Help. }
+    iIntros "!>".
+    iMod (reg_update _ (R_bool minstret_increment) _ b1 with "Hreg Hmi") as "[Hreg Hmi]".
+    iMod (reg_update _ nextPC _ (add_vec_int pc 4) with "Hreg Hnpc") as "[Hreg Hnpc]".
+    iMod (reg_update _ (R_bitvector_64 x2) _ (regval_into_reg (add_vec pc (auipc_off imm_a)))
+            with "Hreg Hx2") as "[Hreg Hx2]".
+    iMod (reg_update _ PC _ (add_vec_int pc 4) with "Hreg Hpc") as "[Hreg Hpc]".
+    unfold sFca, base_upd_a. destruct b1.
+    - iMod (reg_update _ minstret _ (add_vec_int mst0a 1) with "Hreg Hmst") as "[Hreg Hmst]".
+      iMod "Hclose" as "_". iModIntro. unfold set_reg; cbn [sregs mem]. iFrame "Hreg Hmem".
+      iApply ("Hcont" with "Hpc Hx2 Hnpc Hmi Hmst Hpriv Hhs Hmdl Hms Help Hmcinh Hmcfg").
+    - iMod "Hclose" as "_". iModIntro. unfold set_reg; cbn [sregs mem]. iFrame "Hreg Hmem".
+      iApply ("Hcont" with "Hpc Hx2 Hnpc Hmi Hmst Hpriv Hhs Hmdl Hms Help Hmcinh Hmcfg").
+  Qed.
+
+  (* ---------------------------------------------------------------------- *)
+  (* Single-step WP for `ld rd,imm(rs1)` (rs1=rd=x2), via wp_exec_step +     *)
+  (* forward_exec_ld + sFl_eq, discharging Hexec_spc via exec_execute_LOAD_8.*)
+  (* ---------------------------------------------------------------------- *)
+End StepAUIPC.
